cedar-lean/Cedar/Thm/WellTyped/Expr/WF.lean
@@ -96,6 +96,7 @@ theorem well_typed_implies_wf_type
   | hasAttr_record => constructor
   | extHasAttr_entity => constructor
   | extHasAttr_record => constructor
+  | extHasAttr_ff => constructor
   | getAttr_entity _ _ hattrs hattr =>
     simp only [TypedExpr.typeOf]
     simp only [Option.map_eq_some_iff] at hattrs hattr
